\documentclass[12pt]{article}


% ----------------- PAQUETES -----------------
\usepackage[utf8]{inputenc}
\usepackage[spanish]{babel}
\usepackage[margin = 2.54cm]{geometry}
\usepackage{graphicx}
\usepackage{enumitem}
\usepackage{parskip}
\usepackage{bm}
\usepackage{amsmath}
\usepackage{xcolor}


% ----------------- CONFIGURACIONES -----------------
\input{../../../docs/portada-tareas/formato}
\input{../../../docs/portada-tareas/definicion}


% ----------------- PORTADA -----------------
\rutaLogo{../../../docs/img/logo-ista.png}
\tema{\\ \vspace{0.8cm} Taller de ejercicios - Derivadas \\ \vspace{1.5cm}}
\etiquetaAutores{Alumno: }
\alumno{Eduardo Mendieta \vspace{0.8cm}}
\materia{Matemática \vspace{0.8cm}}
\docente{Lcda. Vilma Duchi, Mgtr. \vspace{0.8cm}}
\ciclo{Primer ciclo \vspace{0.8cm}}
\fecha{15/08/2024 \vspace{0.8cm}}
\periodo{Abril 2024 - Agosto 2024}


\begin{document}
    \input{../../../docs/portada-tareas/plantilla}

    \section*{\centering Taller de ejercicios - Derivadas} 
        \textbf{Resolver los siguientes ejercicios:}

    % Actividad 1: ----------------------------------------------------
    \section*{Actividad N°1:}
        \vspace{0.5cm}
        \begin{enumerate}[label=\textbf{\arabic*)}] 
            \hrule\item \[\bm{f(x) = (x^3 + 2x) e^x}\]
                \[f'(x) = (3x^2 + 2)e^x + (x^3 + 2x) e^x\] 
                \[f'(x) = (3x^2e^x + 2e^x) + (x^3e^x + 2xe^x)\] 
                \[f'(x) = x^3e^x + 3x^2e^x + 2xe^x + 2e^x\] 

            \hrule\item \[\bm{y = \frac{x}{e^x}}\]
                \[y' = \frac{e^x - xe^x}{(e^x)^2}\]
                \[y' = \frac{e^x (1 - x)}{(e^x)^2}\]
                \[y' = \frac{1 - x}{e^x}\]

            \hrule\item \[\bm{g(x) = \frac{1 + 2x}{3 - 4x}}\]
                \[g'(x) = \frac{2(3 - 4x) - (1 + 2x)(-4)}{(3 - 4x)^2}\]
                \[g'(x) = \frac{6 - 8x + 4 + 8x}{(3 - 4x)^2}\]
                \[g'(x) = \frac{10 }{(3 - 4x)^2}\]

            \hrule\item \[\bm{H(u) = (u - \sqrt{u})(u + \sqrt{u})} = (u - u^{1/2})(u + u^{1/2})\]
                \[H'(u) = \left(1 - \frac{u^{-1/2}}{2}\right)(u + u^{1/2}) + (u - u^{1/2})\left(1 + \frac{u^{-1/2}}{2}\right)\]
                \[H'(u) = \left(1 - \frac{1}{2\sqrt{u}}\right)(u + \sqrt{u}) + (u - \sqrt{u})\left(1 + \frac{1}{2\sqrt{u}}\right)\]
                \[H'(u) = u - \frac{u}{2\sqrt{u}} + \sqrt{u} - \frac{1}{2} + u + \frac{u}{2\sqrt{u}} - \sqrt{u} - \frac{1}{2}\]
                \[H'(u) = 2u - 1\]

            \newpage
            \hrule\item \[\bm{J(v) = (v^3 - 2v)(v^{-4} + v^{-2})} = v^{-1} + v - 2v^{-3} - 2v^{-1} = -v^{-1} + v - 2v^{-3}\]
                \[J'(v) = v^{-2} + 1 + 6v^{-4}\]
                \[J'(v) = \frac{6}{v^4} + \frac{1}{v^2} + 1\]

            \hrule\item \[\bm{F(y) = \left(\frac{1}{y^2} - \frac{3}{y^4}\right)(y + 5y^3)} = \frac{1}{y} + 5y - \frac{3}{y^3} - \frac{15}{y} = 5y - \frac{3}{y^3} - \frac{14}{y}\]
                \[F(y) = 5y - 3y^{-3} - 14y^{-1}\]
                \[F'(y) = 5 + 9y^{-4} + 14y^{-2}\]
                \[F'(y) = \frac{9}{y^4} + \frac{14}{y^2} + 5\]

            \hrule\item \[\bm{f(z) = (1 - e^z)(z + e^z)} = z + e^z - ze^z - e^{2z}\]
                \[f'(z) = 1 + e^z - (e^z + ze^z) - (2e^{2z})\]
                \[f'(z) = 1 + e^z - e^z - ze^z -2e^{2z}\]
                \[f'(z) = -2e^{2z} - ze^z + 1\]

            \hrule\item \[\bm{y = \frac{x^3}{1 - x^2}}\]
                \[y' = \frac{3x^2 (1 - x^2) - x^3(- 2x)}{(1 - x^2)^2}\]
                \[y' = \frac{3x^2 - 3x^4 + 2x^4}{(1 - x^2)^2}\]
                \[y' = \frac{3x^2 - x^4}{(1 - x^2)^2}\]


            \hrule\item \[\bm{y = \frac{t^2 + 2}{t^4 - 3t^2 + 1}}\]
                \[y' = \frac{2t(t^4 - 3t^2 + 1) - (t^2 + 2)(4t^3 - 6t)}{(t^4 - 3t^2 + 1)^2}\]
                \[y' = \frac{2t^5 - 6t^3 + 2t - (4t^5 - 6t^3 + 8t^3 - 12t)}{(t^4 - 3t^2 + 1)^2}\]
                \[y' = \frac{2t^5 - 6t^3 + 2t - 4t^5 + 6t^3 - 8t^3 + 12t}{(t^4 - 3t^2 + 1)^2}\]
                \[y' = \frac{-2t^5 - 8t^3 + 14t}{(t^4 - 3t^2 + 1)^2}\]

            \hrule\item \[\bm{y = e^p(p + p \sqrt{p})} = e^p(p + pp^{1/2}) = e^p(p + p^{3/2})\]
                \[y' = e^p(p + p^{3/2}) + e^p\left(1 + \frac{3p^{1/2}}{2}\right)\]
                \[y' = e^p p + e^p p^{3/2} + e^p + \frac{3e^p p^{1/2}}{2}\]
                \[y' = e^p p + e^p \sqrt{p^3} + \frac{3e^p \sqrt{p}}{2} + e^p\]


            \hrule\item \[\bm{y = \frac{v^3 - 2v \sqrt{v}}{v}} = \frac{v(v^2 - 2v^{1/2})}{v} = v^2 - 2v^{1/2}\]
                \[y' = 2v - \frac{1}{\sqrt{v}}\]

            \hrule\item \[\bm{f(t) = \frac{2t}{2 + \sqrt{t}}}\]
                \[f'(t) = \frac{2(2 + t^{1/2}) - 2t(\frac{t^{-1/2}}{2})}{(2 + \sqrt{t})^2}\]
                \[f'(t) = \frac{4 + 2t^{1/2} - t^{1/2}}{(2 + \sqrt{t})^2}\]
                \[f'(t) = \frac{4 + t^{1/2}}{(2 + \sqrt{t})^2}\]
                \[f'(t) = \frac{4 + \sqrt{t}}{(2 + \sqrt{t})^2}\]

            \hrule\item \[\bm{f(x) = \frac{A}{B + Ce^x}}\]
                \[f'(x) = \frac{- A(Ce^x)}{(B + Ce^x)^2}\]
                \[f'(x) = \frac{- ACe^x}{(B + Ce^x)^2}\]

            \hrule\item \[\bm{g(x) = \sqrt{x} e^x}\]
                \[g'(x) = \left(\frac{x^{-1/2}}{2} e^x\right) + x^{1/2} e^x\]
                \[g'(x) = \frac{e^x}{2\sqrt{x}} + e^x \sqrt{x}\]

            \hrule\item \[\bm{y = \frac{e^x}{1 - e^x}}\]
                \[y' = \frac{e^x(1 - e^x) - e^x(-e^x)}{(1 - e^x)^2}\]
                \[y' = \frac{e^x - e^{2x} + e^{2x}}{(1 - e^x)^2}\]
                \[y' = \frac{e^x}{(1 - e^x)^2}\]

            \hrule\item \[\bm{G(x) = \frac{x^2 - 2}{2x + 1}}\]
            \hrule\item \[\bm{y = \frac{x + 1}{x^3 + x - 2}}\]
            \hrule\item \[\bm{y = \frac{t}{(t - 1)^2}}\]
            \hrule\item \[\bm{y = \frac{1}{s + ke^s}}\]
            \hrule\item \[\bm{z = w^{3/2} (w + ce^w)}\]
            \hrule\item \[\bm{g(t) = \frac{t - \sqrt{t}}{t^{1/3}}}\]
            \hrule\item \[\bm{f(x) = \frac{1 - xe^x}{x + e^x}}\]
        \end{enumerate}


    % Actividad 2: ----------------------------------------------------
    \section*{Actividad N°2:}
        \vspace{0.5cm}
        \begin{enumerate}[label=\textbf{\arabic*)}] 
            \hrule\item \[\bm{f(x) = 3x^2 - 2\cos{x}}\]
            \hrule\item \[\bm{f(x) = \sqrt{x}\sen{x}}\]
            \hrule\item \[\bm{f(x) = \sen{x} + \frac{1}{2}\cot{x}}\]
            \hrule\item \[\bm{y = 2\sec{x} - \csc{x} }\]
            \hrule\item \[\bm{y = \sec{\theta}\tan{\theta}}\]
            \hrule\item \[\bm{g(\theta) = e^{\theta}(\tan{\theta} - \theta)}\]
            \hrule\item \[\bm{y = c\cos{t} + t^2 \sen{t}}\]
            \hrule\item \[\bm{f(t) = \frac{\cot{t}}{e^t}}\]
            \hrule\item \[\bm{y = \frac{x}{2 - \tan{x}}}\]
            \hrule\item \[\bm{y = \sen{\theta} \cos{\theta}}\]
            \hrule\item \[\bm{f(\theta) = \frac{\sec{\theta}}{1 + \sec{\theta}}}\]
            \hrule\item \[\bm{y = \frac{\cos{x}}{1 - \sen{x}}}\]
            \hrule\item \[\bm{y = \frac{t \sen{t}}{1 + t}}\]
            \hrule\item \[\bm{y = \frac{1 - \sec{x}}{\tan{x}}}\]
            \hrule\item \[\bm{f(x) = xe^x \csc{x}}\]
            \hrule\item \[\bm{y = x^2 \sen{x}\tan{x}}\]
        \end{enumerate}

\end{document}